Calls and returns with protected stack.

ifc/common.v
@@ -32,3 +32,57 @@ Canonical call_frame_eqType :=
   Eval hnf in EqType call_frame call_frame_eqMixin.
 
 End CallFrame.
+
+Fixpoint reap T p (s : seq T) : seq T :=
+  if s is x :: s' then
+    if p x then s else reap p s'
+  else [::].
+
+Section Indist.
+
+Context {T : eqType} {L : labType}.
+Variable t : T -> L.
+
+Local Open Scope label_scope.
+
+Definition indist rs (ra1 ra2 : T) :=
+  (t ra1 ⊑ rs) || (t ra2 ⊑ rs) ==> (ra1 == ra2).
+
+CoInductive indist_spec rs ra1 ra2 : Prop :=
+| IndistLow of t ra1 ⊑ rs & t ra2 ⊑ rs & ra1 = ra2
+| IndistHigh of ~~ (t ra1 ⊑ rs) & ~~ (t ra2 ⊑ rs).
+
+Lemma indistP rs ra1 ra2 :
+  reflect (indist_spec rs ra1 ra2) (indist rs ra1 ra2).
+Proof.
+rewrite /indist; apply/(iffP idP).
+  have [hi /eqP <-|lo1] /= := boolP (t ra1 ⊑ rs); first by constructor.
+  have [hi /eqP e|lo2 _] /= := boolP (t ra2 ⊑ rs).
+    by rewrite e hi in lo1.
+  by apply: IndistHigh.
+case=> [-> -> -> //=|hi1 hi2].
+by rewrite -[X in X ==> _]negbK negb_or hi1 hi2.
+Qed.
+
+Lemma indist_refl rl : reflexive (indist rl).
+Proof. by move=> ra; rewrite /indist eqxx implybT. Qed.
+
+Lemma indist_sym rl : symmetric (indist rl).
+Proof. by move=> ra1 ra2; rewrite /indist orbC eq_sym. Qed.
+
+Lemma indist_trans rl : transitive (indist rl).
+Proof.
+move=> ra2 ra1 ra3; rewrite /indist => e1 e2.
+apply/implyP=> /orP [e|e].
+  by move: e1 e2; rewrite e /= => /eqP <-; rewrite e => /eqP ->.
+by move: e2 e1; rewrite e orbT /= => /eqP ->; rewrite e orbT /= => /eqP ->.
+Qed.
+
+End Indist.
+
+Fixpoint indist_seq T (R : T -> T -> Prop) (s1 s2 : seq T) :=
+  match s1, s2 with
+  | x1 :: s1', x2 :: s2' => R x1 x2 /\ indist_seq R s1' s2'
+  | [::], [::] => True
+  | _, _ => False
+  end.
