ifc/abstract.v
@@ -14,8 +14,12 @@ Import DoNotation.
 Variable L : labType.
 Variable mt : machine_types.
 Variable mops : machine_ops mt.
-Variable r_arg : reg mt.
+Variable r_arg1 : reg mt.
+Variable r_arg2 : reg mt.
+Variable r_ret : reg mt.
 Variable output_addr : mword mt.
+Variable call_addr : mword mt.
+Variable return_addr : mword mt.
 
 Local Notation word := (mword mt).
 Local Notation atom := (atom word L).
@@ -89,11 +93,26 @@ Definition step s : option (state * option atom):=
     else None
   else if pc == output_addr then
     do! raddr <- regs ra;
-    do! out   <- regs r_arg;
+    do! out   <- regs r_arg1;
     let r_pc  := taga raddr in
     let r_out := taga out in
     Some (State mem regs raddr stk,
           Some (vala out)@(r_pc ⊔ r_out))
+  else if pc == call_addr then
+    do! caller_pc <- regs ra;
+    do! called_pc <- regs r_arg1;
+    do! ret_lab   <- regs r_arg2;
+    Some (State mem regs
+                (vala called_pc)@(taga called_pc ⊔ taga caller_pc)
+                (CallFrame caller_pc (taga ret_lab) regs :: stk), None)
+  else if pc == return_addr then
+    if stk is cf :: stk' then
+      do! retv <- regs r_ret;
+      if lpc ⊔ taga retv ⊑ taga (cf_pc cf) ⊔ (cf_lab cf) then
+        do! rs' <- updm (cf_regs cf) r_ret (vala retv)@(cf_lab cf);
+        Some (State mem rs' (cf_pc cf) stk', None)
+      else None
+    else None
   else None.
 
 Fixpoint stepn n s :=
