ifc/symbolic.v
@@ -17,9 +17,12 @@ Local Open Scope label_scope.
 Variable L : labType.
 Variable mt : machine_types.
 Variable mops : machine_ops mt.
-Variable r_arg : reg mt.
+Variable r_arg1 : reg mt.
+Variable r_arg2 : reg mt.
 Variable r_ret : reg mt.
 Variable output_addr : mword mt.
+Variable call_addr : mword mt.
+Variable return_addr : mword mt.
 
 Inductive mem_tag :=
 | MemInstr
@@ -117,7 +120,7 @@ Implicit Types st : state.
 
 Definition output_fun st : option state :=
   do! raddr <- regs st ra;
-  do! out   <- regs st r_arg;
+  do! out   <- regs st r_arg1;
   let r_pc  := taga raddr in
   let r_out := taga out in
   Some (State (mem st) (regs st) (vala raddr)@(taga raddr)
@@ -126,8 +129,35 @@ Definition output_fun st : option state :=
                  call_stack := call_stack (internal st)
               |}).
 
+Definition call_fun st : option state :=
+  do! caller_pc <- regs st ra;
+  do! called_pc <- regs st r_arg1;
+  do! ret_lab   <- regs st r_arg2;
+  Some (State (mem st) (regs st)
+              (vala called_pc)@(taga called_pc ⊔ taga caller_pc)
+              {| outputs := outputs (internal st);
+                 call_stack :=
+                   CallFrame caller_pc (taga ret_lab) (regs st)
+                   :: call_stack (internal st)
+              |}).
+
+Definition return_fun st : option state :=
+  if call_stack (internal st) is cf :: stk then
+    do! retv <- regs st r_ret;
+    if taga (pc st) ⊔ taga retv ⊑ taga (cf_pc cf) ⊔ (cf_lab cf) then
+      do! rs' <- updm (cf_regs cf) r_ret (vala retv)@(cf_lab cf);
+      Some (State (mem st) rs' (cf_pc cf)
+                  {| outputs := outputs (internal st);
+                     call_stack := stk |})
+    else None
+  else None.
+
 Definition ifc_syscalls : syscall_table mt :=
-  [partmap (output_addr, (Syscall tt output_fun))].
+  [partmap
+     (output_addr, (Syscall tt output_fun));
+     (call_addr, (Syscall tt call_fun));
+     (return_addr, (Syscall tt return_fun))
+  ].
 
 Local Notation step  := (@Symbolic.step mt mops sym_ifc ifc_syscalls).
 Local Notation ratom := (atom (mword mt) (tag_type ifc_tags R)).
